\[\mathop{L^{(\alpha)}_{n}\/}\nolimits\!\left(x\right)=\frac{\left(\alpha+1%
\right)_{n}}{n!}\mathop{M\/}\nolimits\!\left(-n,\alpha+1,x\right)=\frac{(-1)^{%
n}}{n!}\mathop{U\/}\nolimits\!\left(-n,\alpha+1,x\right)=\frac{\left(\alpha+1%
\right)_{n}}{n!}x^{-\frac{1}{2}(\alpha+1)}e^{\frac{1}{2}x}\mathop{M_{n+\frac{1%
}{2}(\alpha+1),\frac{1}{2}\alpha}\/}\nolimits\!\left(x\right)=\frac{(-1)^{n}}{%
n!}x^{-\frac{1}{2}(\alpha+1)}e^{\frac{1}{2}x}\mathop{W_{n+\frac{1}{2}(\alpha+1%
),\frac{1}{2}\alpha}\/}\nolimits\!\left(x\right).\]