\[\mathop{\mathrm{Ai}\/}\nolimits'\!\left(z\right)=-\pi^{-1}(z/\sqrt{3})\mathop{%
K_{\pm 2/3}\/}\nolimits\!\left(\zeta\right)=(z/3)\left(\mathop{I_{2/3}\/}%
\nolimits\!\left(\zeta\right)-\mathop{I_{-2/3}\/}\nolimits\!\left(\zeta\right)%
\right)=\tfrac{1}{2}(z/\sqrt{3})e^{-\pi i/6}\mathop{{H^{(1)}_{2/3}}\/}%
\nolimits\!\left(\zeta e^{\pi i/2}\right)=\tfrac{1}{2}(z/\sqrt{3})e^{-5\pi i/6%
}\mathop{{H^{(1)}_{-2/3}}\/}\nolimits\!\left(\zeta e^{\pi i/2}\right)=\tfrac{1%
}{2}(z/\sqrt{3})e^{\pi i/6}\mathop{{H^{(2)}_{2/3}}\/}\nolimits\!\left(\zeta e^%
{-\pi i/2}\right)=\tfrac{1}{2}(z/\sqrt{3})e^{5\pi i/6}\mathop{{H^{(2)}_{-2/3}}%
\/}\nolimits\!\left(\zeta e^{-\pi i/2}\right),\]