\[\mathop{\mathbf{F}\/}\nolimits\!\left({a+\lambda,b-\lambda\atop c};\tfrac{1}{2%
}-\tfrac{1}{2}z\right)=2^{(a+b-1)/2}\frac{(z+1)^{(c-a-b-1)/2}}{(z-1)^{c/2}}%
\sqrt{\zeta\mathop{\sinh\/}\nolimits\zeta}\left(\lambda+\tfrac{1}{2}a-\tfrac{1%
}{2}b\right)^{1-c}\left(\mathop{I_{c-1}\/}\nolimits\!\left((\lambda+\tfrac{1}{%
2}a-\tfrac{1}{2}b)\zeta\right)(1+\mathop{O\/}\nolimits(\lambda^{-2}))+\frac{%
\mathop{I_{c-2}\/}\nolimits\!\left((\lambda+\tfrac{1}{2}a-\tfrac{1}{2}b)\zeta%
\right)}{2\lambda+a-b}\left(\left(c-\tfrac{1}{2}\right)\left(c-\tfrac{3}{2}%
\right)\left(\frac{1}{\zeta}-\mathop{\coth\/}\nolimits\zeta\right)+\tfrac{1}{2%
}(2c-a-b-1)(a+b-1)\mathop{\tanh\/}\nolimits\!\left(\tfrac{1}{2}\zeta\right)+%
\mathop{O\/}\nolimits(\lambda^{-2})\right)\right),\]