\[\mathop{F\/}\nolimits\!\left({a,b-\lambda\atop c+\lambda};-z\right)=2^{b-c+(1/%
2)}\left(\frac{z+1}{2\sqrt{z}}\right)^{\lambda}\left(\lambda^{a/2}\mathop{U\/}%
\nolimits\!\left(a-\tfrac{1}{2},-\alpha\sqrt{\lambda}\right)\left((1+z)^{c-a-b%
}z^{1-c}\left(\frac{\alpha}{z-1}\right)^{1-a}+\mathop{O\/}\nolimits(\lambda^{-%
1})\right)+\frac{\lambda^{\ifrac{(a-1)}{2}}}{\alpha}\mathop{U\/}\nolimits\!%
\left(a-\tfrac{3}{2},-\alpha\sqrt{\lambda}\right)\left((1+z)^{c-a-b}z^{1-c}%
\left(\frac{\alpha}{z-1}\right)^{1-a}-2^{c-b-(\ifrac{1}{2})}\left(\frac{\alpha%
}{z-1}\right)^{a}+\mathop{O\/}\nolimits(\lambda^{-1})\right)\right),\]