\[(z+1)^{3\lambda/2}(2\lambda)^{c-1}\mathop{\mathbf{F}\/}\nolimits\!\left({a+%
\lambda,b+2\lambda\atop c};-z\right)={\lambda^{-1/3}\left(e^{\pi i(a-c+\lambda%
+(1/3))}\mathop{\mathrm{Ai}\/}\nolimits\!\left(e^{-\ifrac{2\pi i}{3}}\lambda^{%
\ifrac{2}{3}}\beta^{2}\right)+e^{\pi i(c-a-\lambda-(1/3))}\mathop{\mathrm{Ai}%
\/}\nolimits\!\left(e^{\ifrac{2\pi i}{3}}\lambda^{\ifrac{2}{3}}\beta^{2}\right%
)\right)\left(a_{0}(\zeta)+\mathop{O\/}\nolimits(\lambda^{-1})\right)}+\lambda%
^{-2/3}\left(e^{\pi i(a-c+\lambda+(2/3))}\mathop{\mathrm{Ai}\/}\nolimits'\!%
\left(e^{-\ifrac{2\pi i}{3}}\lambda^{\ifrac{2}{3}}\beta^{2}\right)+e^{\pi i(c-%
a-\lambda-(2/3))}\mathop{\mathrm{Ai}\/}\nolimits'\!\left(e^{\ifrac{2\pi i}{3}}%
\lambda^{\ifrac{2}{3}}\beta^{2}\right)\right)\left(a_{1}(\zeta)+\mathop{O\/}%
\nolimits(\lambda^{-1})\right),\]