\[\mathop{F\/}\nolimits\!\left({\frac{1}{2}+\lambda,-\frac{1}{2}-\nu\atop 1+%
\lambda+\mu};z\right)\mathop{F\/}\nolimits\!\left({\frac{1}{2}-\lambda,\frac{1%
}{2}+\nu\atop 1+\nu+\mu};1-z\right)+\mathop{F\/}\nolimits\!\left({\frac{1}{2}+%
\lambda,\frac{1}{2}-\nu\atop 1+\lambda+\mu};z\right)\mathop{F\/}\nolimits\!%
\left({-\frac{1}{2}-\lambda,\frac{1}{2}+\nu\atop 1+\nu+\mu};1-z\right)-\mathop%
{F\/}\nolimits\!\left({\frac{1}{2}+\lambda,\frac{1}{2}-\nu\atop 1+\lambda+\mu}%
;z\right)\mathop{F\/}\nolimits\!\left({\frac{1}{2}-\lambda,\frac{1}{2}+\nu%
\atop 1+\nu+\mu};1-z\right)=\frac{\mathop{\Gamma\/}\nolimits\!\left(1+\lambda+%
\mu\right)\mathop{\Gamma\/}\nolimits\!\left(1+\nu+\mu\right)}{\mathop{\Gamma\/%
}\nolimits\!\left(\lambda+\mu+\nu+\frac{3}{2}\right)\mathop{\Gamma\/}\nolimits%
\!\left(\frac{1}{2}+\nu\right)},\]